Refine Imp

Vol1/Imp.v
@@ -166,3 +166,225 @@ Proof.
 Qed.
 
 End AExp.
+
+Definition state := total_map nat.
+
+Inductive aexp : Type :=
+  | ANum (n : nat)
+  | AId (x : string) (* <--- NEW *)
+  | APlus (a1 a2 : aexp)
+  | AMinus (a1 a2 : aexp)
+  | AMult (a1 a2 : aexp).
+
+Definition W : string := "W".
+Definition X : string := "X".
+Definition Y : string := "Y".
+Definition Z : string := "Z".
+
+Inductive bexp : Type :=
+  | BTrue
+  | BFalse
+  | BEq (a1 a2 : aexp)
+  | BNeq (a1 a2 : aexp)
+  | BLe (a1 a2 : aexp)
+  | BGt (a1 a2 : aexp)
+  | BNot (b : bexp)
+  | BAnd (b1 b2 : bexp).
+
+Coercion AId : string >-> aexp.
+Coercion ANum : nat >-> aexp.
+
+Declare Custom Entry com.
+Declare Scope com_scope.
+Notation "<{ e }>" := e (at level 0, e custom com at level 99) : com_scope.
+Notation "( x )" := x (in custom com, x at level 99) : com_scope.
+Notation "x" := x (in custom com at level 0, x constr at level 0) : com_scope.
+Notation "f x .. y" := (.. (f x) .. y)
+                  (in custom com at level 0, only parsing,
+                  f constr at level 0, x constr at level 9,
+                  y constr at level 9) : com_scope.
+Notation "x + y" := (APlus x y) (in custom com at level 50, left associativity).
+Notation "x - y" := (AMinus x y) (in custom com at level 50, left associativity).
+Notation "x * y" := (AMult x y) (in custom com at level 40, left associativity).
+Notation "'true'" := true (at level 1).
+Notation "'true'" := BTrue (in custom com at level 0).
+Notation "'false'" := false (at level 1).
+Notation "'false'" := BFalse (in custom com at level 0).
+Notation "x <= y" := (BLe x y) (in custom com at level 70, no associativity).
+Notation "x > y" := (BGt x y) (in custom com at level 70, no associativity).
+Notation "x = y" := (BEq x y) (in custom com at level 70, no associativity).
+Notation "x <> y" := (BNeq x y) (in custom com at level 70, no associativity).
+Notation "x && y" := (BAnd x y) (in custom com at level 80, left associativity).
+Notation "'~' b" := (BNot b) (in custom com at level 75, right associativity).
+Open Scope com_scope.
+
+(* We can now write 3 + (X × 2) instead of APlus 3 (AMult X 2), and true && ~(X ≤ 4) instead of BAnd 
+true (BNot (BLe X 4)). *)
+
+Fixpoint aeval (st : state) (* <--- NEW *) (a : aexp) : nat :=
+  match a with
+  | ANum n => n
+  | AId x => st x (* <--- NEW *)
+  | <{a1 + a2}> => (aeval st a1) + (aeval st a2)
+  | <{a1 - a2}> => (aeval st a1) - (aeval st a2)
+  | <{a1 * a2}> => (aeval st a1) * (aeval st a2)
+  end.
+
+Fixpoint beval (st : state) (* <--- NEW *) (b : bexp) : bool :=
+  match b with
+  | <{true}> => true
+  | <{false}> => false
+  | <{a1 = a2}> => (aeval st a1) =? (aeval st a2)
+  | <{a1 <> a2}> => negb ((aeval st a1) =? (aeval st a2))
+  | <{a1 <= a2}> => (aeval st a1) <=? (aeval st a2)
+  | <{a1 > a2}> => negb ((aeval st a1) <=? (aeval st a2))
+  | <{~ b1}> => negb (beval st b1)
+  | <{b1 && b2}> => andb (beval st b1) (beval st b2)
+  end.
+
+Definition empty_st := (_ !-> 0).
+
+(* singleton state *)
+Notation "x '!->' v" := (x !-> v ; empty_st) (at level 100).
+
+Inductive com : Type :=
+  | CSkip
+  | CAsgn (x : string) (a : aexp)
+  | CSeq (c1 c2 : com)
+  | CIf (b : bexp) (c1 c2 : com)
+  | CWhile (b : bexp) (c : com).
+
+Notation "'skip'" :=
+    CSkip (in custom com at level 0) : com_scope.
+Notation "x := y" :=
+    (CAsgn x y)
+       (in custom com at level 0, x constr at level 0,
+        y at level 85, no associativity) : com_scope.
+Notation "x ; y" :=
+    (CSeq x y)
+      (in custom com at level 90, right associativity) : com_scope.
+Notation "'if' x 'then' y 'else' z 'end'" :=
+    (CIf x y z)
+      (in custom com at level 89, x at level 99,
+       y at level 99, z at level 99) : com_scope.
+Notation "'while' x 'do' y 'end'" :=
+    (CWhile x y)
+       (in custom com at level 89, x at level 99, y at level 99) : com_scope.
+
+Fixpoint ceval_fun_no_while (st : state) (c : com) : state :=
+  match c with
+    | <{ skip }> =>
+        st
+    | <{ x := a }> =>
+        (x !-> (aeval st a) ; st)
+    | <{ c1 ; c2 }> =>
+        let st' := ceval_fun_no_while st c1 in
+        ceval_fun_no_while st' c2
+    | <{ if b then c1 else c2 end}> =>
+        if (beval st b)
+          then ceval_fun_no_while st c1
+          else ceval_fun_no_while st c2
+    | <{ while b do c end }> =>
+        st (* bogus *)
+  end.
+
+(* Operational Semantics *)
+Reserved Notation
+         "st '=[' c ']=>' st'"
+         (at level 40, c custom com at level 99,
+          st constr, st' constr at next level).
+
+Inductive ceval : com -> state -> state -> Prop :=
+  | E_Skip : forall st,
+      st =[ skip ]=> st
+  | E_Asgn : forall st a n x,
+      aeval st a = n ->
+      st =[ x := a ]=> (x !-> n ; st)
+  | E_Seq : forall c1 c2 st st' st'',
+      st =[ c1 ]=> st' ->
+      st' =[ c2 ]=> st'' ->
+      st =[ c1 ; c2 ]=> st''
+  | E_IfTrue : forall st st' b c1 c2,
+      beval st b = true ->
+      st =[ c1 ]=> st' ->
+      st =[ if b then c1 else c2 end]=> st'
+  | E_IfFalse : forall st st' b c1 c2,
+      beval st b = false ->
+      st =[ c2 ]=> st' ->
+      st =[ if b then c1 else c2 end]=> st'
+  | E_WhileFalse : forall b st c,
+      beval st b = false ->
+      st =[ while b do c end ]=> st
+  | E_WhileTrue : forall st st' st'' b c,
+      beval st b = true ->
+      st =[ c ]=> st' ->
+      st' =[ while b do c end ]=> st'' ->
+      st =[ while b do c end ]=> st''
+
+  where "st =[ c ]=> st'" := (ceval c st st').
+
+Example ceval_example1:
+  empty_st =[
+     X := 2;
+     if (X <= 1)
+       then Y := 3
+       else Z := 4
+     end
+  ]=> (Z !-> 4 ; X !-> 2).
+Proof.
+  apply E_Seq with (X !-> 2).
+  - apply E_Asgn. trivial.
+  - apply E_IfFalse.
+    + trivial.
+    + apply E_Asgn. trivial.
+Qed.
+
+Example ceval_example2:
+  empty_st =[
+    X := 0;
+    Y := 1;
+    Z := 2
+  ]=> (Z !-> 2 ; Y !-> 1 ; X !-> 0).
+Proof.
+  apply E_Seq with (X !-> 0).
+  - apply E_Asgn. trivial.
+  - apply E_Seq with (Y !-> 1; X !-> 0); (* Treat as a whole. *)
+  apply E_Asgn; trivial.
+Qed.
+
+Definition fact_in_coq : com :=
+  <{ Z := X;
+     Y := 1;
+     while Z <> 0 do
+       Y := Y * Z;
+       Z := Z - 1
+     end }>.
+
+(* Write an Imp program that sums the numbers from 1 to X (inclusive: 1 + 2 + ... + X) in the variable Y.  *)
+Definition pup_to_n : com :=
+  <{
+    Y := 0;
+    while X <> 0 do
+      Y := Y + X;
+      X := X - 1
+    end
+  }>.
+
+Theorem pup_to_2_ceval :
+  (X !-> 2) =[
+    pup_to_n
+  ]=> (X !-> 0 ; Y !-> 3 ; X !-> 1 ; Y !-> 2 ; Y !-> 0 ; X !-> 2). 
+  (* can be treated as a reverse-ordered state list? *)
+  (* final, prev1, prev2, initial. *)
+Proof.
+  unfold pup_to_n.
+  apply E_Seq with (Y !-> 0 ; X !-> 2).
+  - apply E_Asgn. trivial.
+  - apply E_WhileTrue with (X !-> 1 ; Y !-> 2 ; Y !-> 0 ; X !-> 2).
+    * trivial.
+    * apply E_Seq with (Y !-> 2; Y !-> 0; X !-> 2); apply E_Asgn; trivial.
+    * apply E_WhileTrue with (X !-> 0 ; Y !-> 3 ; X !-> 1 ; Y !-> 2 ; Y !-> 0 ; X !-> 2).
+      + trivial.
+      + apply E_Seq with (Y !-> 3 ; X !-> 1 ; Y !-> 2 ; Y !-> 0 ; X !-> 2); apply E_Asgn; trivial.
+      + apply E_WhileFalse. trivial.
+Qed.
